Examples/Evm/Contracts/stdlib/ReentrancyGuard.golden.yul
@@ -1,0 +1,33 @@
+object "ReentrancyGuard" {
+  code {
+    switch shr(224, calldataload(0))
+    case 0xa7134f73 {
+      f_ReentrancyGuard_acquire()
+      return(0, 0)
+    }
+    case 0x86d1a69f {
+      f_ReentrancyGuard_release()
+      return(0, 0)
+    }
+    case 0xcf309012 {
+      let _r := f_ReentrancyGuard_locked()
+      mstore(0, _r)
+      return(0, 32)
+    }
+    default {
+      revert(0, 0)
+    }
+    function f_ReentrancyGuard_acquire() {
+      if iszero(eq(sload(0), 0)) {
+        revert(0, 0)
+      }
+      sstore(0, 1)
+    }
+    function f_ReentrancyGuard_release() {
+      sstore(0, 0)
+    }
+    function f_ReentrancyGuard_locked() -> result {
+      result := sload(0)
+    }
+  }
+}
